noActionStacksInIVars/classifiedStep.v
@@ -51,7 +51,7 @@ Inductive prog_step : sHeap -> pool -> pool -> config -> Prop :=
               wf = decomposeWF t E (specRun (ret N1) N0) p ->
               s1' = (wrapActs s1 N1 E (specRun (ret N1) N0) wf) ->
               prog_step h T (tCouple t1 t2) 
-                   (OK h T (tSingleton(tid,unlocked s1', s2, fill E (specJoin (ret N1) M)))) 
+                   (OK h T (tSingleton(2::tid,unlocked s1', s2', fill E (specJoin (ret N1) M)))) 
 |CSpecRB : forall t E' h h' tid T T' E M' N0 s2 s1 s2' t1 t2 TRB, 
             decompose t E' (specRun (raise E) N0)->
             t1 = (tid,(unlocked nil),s2,t) -> t2 = (2::tid,locked s1,s2',M') -> 
@@ -316,14 +316,6 @@ Proof.
   }
 Qed.  
 
-Theorem InL : forall X T1 T2 t, In X T2 t -> In X (Union X T1 T2) t. 
-Proof.
-  intros. apply Union_intror. auto. 
-Qed. 
-
-Hint Resolve InL. 
- 
-Ltac solveSet := try(solve[eauto with sets]); try solve[eapply InL; eauto with sets]. 
 
 Ltac firstActTac H := eapply firstActEq in H;
                      [idtac|apply InL; constructor|solveSet|simpl;try rewrite app_nil_l; eauto|simpl;eauto].
