noActionStacksInIVars/sets.v
@@ -1,30 +1,26 @@
 Require Import Coq.Logic.Classical.
 Require Import Coq.Sets.Ensembles.
 
-Section Ensembles.
-
-Variable U : Type.
-
-Lemma union_empty_r : forall A,
+Lemma union_empty_r : forall U A,
   Union U A (Empty_set U) = A.
 Proof.
-  intros A. apply Extensionality_Ensembles.
+  intros. apply Extensionality_Ensembles.
   split; intros x x_in_one.
   inversion x_in_one as [ _x in_A x_eq | _x false x_eq ].
   auto. inversion false.
   left. auto.
 Qed.
 
-Lemma union_empty_l : forall A, Union U (Empty_set U) A = A. 
+Lemma union_empty_l : forall U A, Union U (Empty_set U) A = A. 
 Proof.
   intros. apply Extensionality_Ensembles. split; intros x x'. 
   inversion x'. inversion H. auto. apply Union_intror. auto. 
 Qed. 
 
-Lemma union_swap : forall A B,
+Lemma union_swap : forall U A B,
   Union U A B = Union U B A.
 
-intros A B.
+intros. 
 apply Extensionality_Ensembles. 
 split; intros x x_in_one;
 destruct x_in_one as [ x x_in_left | x x_in_right ];
@@ -33,10 +29,10 @@ auto using Union_introl, Union_intror.
 Qed.
 
 Lemma disjoint_setminus :
-  forall A B,
+  forall U A B,
     Disjoint U A (Setminus U B A).
 
-  intros A B.
+  intros.
   apply Disjoint_intro. unfold not.
   intros x in_int.
   destruct in_int as [ x x_in_A x_in_setminus ].
@@ -46,10 +42,10 @@ Lemma disjoint_setminus :
 Qed.
 
 Lemma add_add_to_union_couple :
-  forall A x y,
+  forall U A x y,
     (Add U (Add U A x) y) = (Union U A (Couple U y x)).
 
-intros A x y.
+intros.
 apply Extensionality_Ensembles. split; intros z z_in_one.
 destruct z_in_one as [ z' [ z z_in_A | z z_is_x ] | z z_is_y ].
 left. auto. 
@@ -63,10 +59,10 @@ left. right. apply In_singleton.
 Qed.
 
 Lemma couple_swap :
-  forall A B,
+  forall U A B,
     Couple U A B = Couple U B A.
 
-intros A B.
+intros.
 apply Extensionality_Ensembles. split; intros x x_in_one.
 destruct x_in_one. right. left.
 destruct x_in_one. right. left.
@@ -74,11 +70,11 @@ destruct x_in_one. right. left.
 Qed.
 
 Lemma add_subtract :
-  forall A x,
+  forall U A x,
     In U A x ->
     A = Add U (Subtract U A x) x.
 
-intros A x in_A.
+intros.
 apply Extensionality_Ensembles. split; intros y y_in_one.
 assert (x = y \/ x <> y) as [ is_x | not_x ]. apply classic.
 right. subst y. apply In_singleton.
@@ -97,12 +93,6 @@ Proof.
   {subst. assumption. }
 Qed. 
 
-Ltac unfoldSetEq H :=
-  match type of H with
-      |?S1 = ?S2 => apply eqImpliesSameSet in H; unfold Same_set in H; 
-                    unfold Included in *; inversion H
-  end. 
-
 Hint Unfold In. 
 Hint Constructors Singleton Couple. 
 
@@ -119,38 +109,52 @@ Qed.
 
 Theorem SingletonEq : forall (T:Type) (e1 e2 : T), Singleton T e1 = Singleton T e2 -> e1 = e2. 
 Proof.
-  intros. unfoldSetEq H. assert(Ensembles.In T (Singleton T e1) e1). auto. apply H0 in H2. 
+  intros. apply eqImpliesSameSet in H. unfold Same_set in H. unfold Included in *. 
+  inversion H. assert(Ensembles.In T (Singleton T e1) e1). auto. apply H0 in H2. 
   inversion H2. reflexivity. Qed. 
  
 Theorem UnionEqSingleton : forall (T:Type) S e1 e2, 
                              Union T S (Singleton T e1) = Singleton T e2 ->
                              e1 = e2. 
 Proof.
-  intros. unfoldSetEq H. clear H. assert(In T (Union T S(Singleton T e1)) e1). 
-  apply Union_intror. constructor. apply H0 in H. inversion H. 
+  intros. apply eqImpliesSameSet in H. unfold Same_set in H. unfold Included in *. 
+  inversion H. assert(In T (Union T S(Singleton T e1)) e1). 
+  apply Union_intror. constructor. apply H0 in H2. inversion H2. 
   reflexivity. Qed. 
+
+Theorem InL : forall X T1 T2 t, In X T2 t -> In X (Union X T1 T2) t. 
+Proof.
+  intros. apply Union_intror. auto. 
+Qed. 
+
+Hint Resolve InL. 
+ 
+Ltac solveSet := try(solve[eauto with sets]); try solve[eapply InL; eauto with sets]. 
+
+Ltac eqSets := apply Extensionality_Ensembles; unfold Same_set; unfold Included; split; intros. 
+
 
 Theorem disjointUnionEqSingleton : forall (T:Type) S e1 e2, 
                                      Disjoint T S (Singleton T e1) ->
                                      Union T S (Singleton T e1) = Singleton T e2 ->
                                      e1 = e2 /\ S = Empty_set T. 
 Proof.
-  intros. unfoldSetEq H0. clear H0. inversion H. split.
+  intros. apply eqImpliesSameSet in H0. unfold Same_set in *. unfold Included in *. 
+  inversion H0. inversion H. split.
   {assert(In T (Union T S (Singleton T e1)) e1). apply Union_intror. 
-   constructor. apply H1 in H3. inversion H3. reflexivity. }
-  {assert(In T (Singleton T e2) e2). constructor. apply H2 in H3. 
-   inversion H3. 
-   {assert(In T (Union T S (Singleton T e1)) e1). apply Union_intror. 
-    constructor. apply H1 in H6. inversion H6. subst. inversion H. 
-    assert(In T (Intersection T S (Singleton T e1)) e1). constructor; assumption. 
-    apply H5 in H7. inversion H7. }
+   constructor. apply H1 in H4. inversion H4. reflexivity. }
+  {assert(In T (Singleton T e2) e2). constructor. apply H2 in H4. inversion H4. 
+   {assert(In T (Union T S (Singleton T e1)) e1). solveSet. apply H1 in H7. 
+    inversion H7. subst. inversion H. 
+    assert(In T (Intersection T S (Singleton T e1)) e1). solveSet. 
+    apply H6 in H8. contradiction. }
    {subst. apply Extensionality_Ensembles. unfold Same_set. unfold Included. 
     split; intros. 
-    {assert(In T (Union T S (Singleton T e1)) x). apply Union_introl. assumption. 
-     apply H1 in H6. inversion H6. subst. inversion H4. subst. 
-     assert(In T (Intersection T S(Singleton T x)) x). constructor; assumption. 
-     apply H0 in H7. inversion H7. }
-    {inversion H5. }
+    {assert(In T (Union T S (Singleton T e1)) x). solveSet. 
+     apply H1 in H7. inversion H7. subst. inversion H5. subst. 
+     assert(In T (Intersection T S(Singleton T x)) x). solveSet. 
+     apply H3 in H8. contradiction. }
+    {inversion H6. }
    }
   }
 Qed. 
@@ -158,8 +162,11 @@ Qed.
 Theorem AddEqCouple : forall T S e e1 e2, Add T S e = Couple T e1 e2 ->
                                           e = e1 \/ e = e2. 
 Proof.
-  intros. unfold Add in H. unfoldSetEq H. assert(Ensembles.In T (Union T S (Singleton T e)) e).
-  apply Union_intror. constructor. apply H0 in H2. inversion H2. auto. auto. Qed. 
+  intros. unfold Add in H. apply eqImpliesSameSet in H. unfold Same_set in *. 
+  unfold Included in *. inversion H. 
+  assert(Ensembles.In T (Union T S (Singleton T e)) e). solveSet. 
+  apply H0 in H2. inversion H2; auto. 
+Qed. 
 
 Theorem AddEqSingleton : forall T S e e', Add T S e = Singleton T e' -> e = e'. 
 Proof.
@@ -215,5 +222,43 @@ Proof.
    apply Union_intror. auto. constructor. apply Union_intror. auto. }
 Qed. 
 
-End Ensembles.
+
+Theorem UnionSwapR : forall X T t1 t2 t3,
+                       Union X (Union X T (Singleton X t1)) (Couple X t2 t3) = 
+                       Union X (Union X T (Singleton X t3)) (Couple X t2 t1). 
+Proof.
+  intros. eqSets. 
+  {inversion H; inversion H0; subst; solveSet. inversion H2; subst; solveSet. }
+  {inversion H; inversion H0; solveSet. inversion H2; subst. solveSet. }
+Qed. 
+
+Theorem UnionSwapL : forall X T t1 t2 t3,
+                       Union X (Union X T (Singleton X t1)) (Couple X t2 t3) = 
+                       Union X (Union X T (Singleton X t2)) (Couple X t1 t3). 
+Proof.
+  intros. eqSets. 
+  {inversion H; inversion H0; solveSet. inversion H2; solveSet. }
+  {inversion H; inversion H0; solveSet. inversion H2; solveSet. }
+Qed.
+
+Theorem pullOutR : forall X T t1 t2, 
+                     Union X T (Couple X t1 t2) = 
+                     Union X (Union X T (Singleton X t1)) (Singleton X t2). 
+Proof.
+  intros. eqSets. 
+  {inversion H; solveSet. inversion H0; solveSet. }
+  {inversion H; solveSet; inversion H0; solveSet. inversion H2; solveSet. }
+Qed. 
+
+
+Theorem pullOutL : forall X T t1 t2, 
+                     Union X T (Couple X t1 t2) = 
+                     Union X (Union X T (Singleton X t2)) (Singleton X t1). 
+Proof.
+  intros. eqSets. 
+  {inversion H; solveSet. inversion H0; solveSet. }
+  {inversion H; solveSet; inversion H0; solveSet. inversion H2; solveSet. }
+Qed. 
+
+
 
